proof/agp32_MEM_CorrectScript.sml
@@ -452,29 +452,32 @@ Theorem agp32_Rel_ag32_data_addr_correct_read_mem:
     is_mem fext_accessor_circuit (agp32 fext fbits) fext ==>
     is_sch I (agp32 fext fbits) a ==>
     Rel I (fext t) (agp32 fext fbits (t-1)) (agp32 fext fbits t) a t ==>
-    (agp32 fext fbits t).MEM.MEM_opc = 4w ==>
-    enable_stg 4 (agp32 fext fbits t) ==>
+    I (5, SUC t) <> NONE ==>
+    (agp32 fext fbits (SUC t)).WB.WB_opc = 4w ==>
     align_addr (agp32 fext fbits (SUC t)).data_addr =
     mem_data_addr (FUNPOW Next (THE (I (5,SUC t)) − 1) a)
 Proof
-  rw [] >> Q.ABBREV_TAC `s = agp32 fext fbits t` >>
-  `(agp32 fext fbits (SUC t)).data_addr = (agp32_next_state (fext t) s s).data_addr`
-    by fs [agp32_data_addr_wstrb_wdata_updated_by_agp32_next_state] >>
-  `(fext t).error = 0w` by fs [is_mem_def,mem_no_errors_def] >>
-  `s.MEM.MEM_read_mem` by METIS_TAC [Abbr `s`,agp32_MEM_read_mem_MEM_opc_4w_5w] >>
-  `enable_stg 5 s` by fs [Abbr `s`,enable_stg_def,agp32_MEM_state_flag_eq_WB_state_flag] >>
-  `I' (5,SUC t) = I' (4,t)` by fs [is_sch_def,is_sch_writeback_def] >>
-  `s.state = 0w`
-    by (fs [Abbr `s`,enable_stg_def] >> Cases_on_word_value `(agp32 fext fbits t).state` >>
-        METIS_TAC [agp32_MEM_state_flag_and_state,agp32_state_impossible_values]) >>
-  `(fext t).ready`
-    by (fs [Abbr `s`,enable_stg_def] >> METIS_TAC [agp32_MEM_state_flag_and_fext_ready]) >>
-  fs [agp32_next_state_def] >>
-  `~s.MEM.MEM_isInterrupt` by fs [Abbr `s`,agp32_MEM_read_mem_others_F] >> fs [] >>
-  Cases_on `I' (4,t) = NONE` >-
-   fs [Rel_def,Inv_Rel_def] >>
-  `opc (FUNPOW Next (THE (I' (4,t)) − 1) a) = 4w` by fs [Rel_def,MEM_Rel_def] >>           
-  fs [mem_data_addr_def,Rel_def,MEM_Rel_def]
+  rw [] >> Cases_on `enable_stg 5 (agp32 fext fbits t)` >-
+   (Q.ABBREV_TAC `s = agp32 fext fbits t` >>              
+    `(agp32 fext fbits (SUC t)).data_addr = (agp32_next_state (fext t) s s).data_addr`
+      by fs [agp32_data_addr_wstrb_wdata_updated_by_agp32_next_state] >>
+    `(fext t).error = 0w` by fs [is_mem_def,mem_no_errors_def] >>
+    `s.MEM.MEM_opc = 4w` by fs [agp32_WB_opc_MEM_opc_when_WB_enabled,Abbr `s`] >>
+    `s.MEM.MEM_read_mem` by METIS_TAC [Abbr `s`,agp32_MEM_read_mem_MEM_opc_4w_5w] >>
+    `I' (5,SUC t) = I' (4,t)` by fs [is_sch_def,is_sch_writeback_def] >>
+    `s.state = 0w`
+      by (fs [Abbr `s`,enable_stg_def] >> Cases_on_word_value `(agp32 fext fbits t).state` >>
+          METIS_TAC [agp32_WB_state_flag_and_state,agp32_state_impossible_values]) >>
+    `(fext t).ready`
+      by (fs [Abbr `s`,enable_stg_def] >> METIS_TAC [agp32_WB_state_flag_and_fext_ready]) >>
+    fs [agp32_next_state_def] >>
+    `~s.MEM.MEM_isInterrupt` by fs [Abbr `s`,agp32_MEM_read_mem_others_F] >> fs [] >>
+    `opc (FUNPOW Next (THE (I' (4,t)) − 1) a) = 4w` by fs [Rel_def,MEM_Rel_def] >>
+    fs [mem_data_addr_def,Rel_def,MEM_Rel_def]) >>
+  `(agp32 fext fbits (SUC t)).data_addr = (agp32 fext fbits t).data_addr` by cheat >>
+  `I' (5,SUC t) = I' (5,t)` by fs [is_sch_def,is_sch_disable_def] >>
+  `(agp32 fext fbits t).WB.WB_opc = 4w` by fs [agp32_WB_opc_unchanged_when_WB_disabled] >>
+  fs [Rel_def,MEM_req_rel_def]
 QED
 
 (** LoadMemByte **)
@@ -483,52 +486,31 @@ Theorem agp32_Rel_ag32_data_addr_correct_read_mem_byte:
     is_mem fext_accessor_circuit (agp32 fext fbits) fext ==>
     is_sch I (agp32 fext fbits) a ==>
     Rel I (fext t) (agp32 fext fbits (t-1)) (agp32 fext fbits t) a t ==>
-    (agp32 fext fbits t).MEM.MEM_opc = 5w ==>
-    enable_stg 4 (agp32 fext fbits t) ==>
+    I (5, SUC t) <> NONE ==>
+    (agp32 fext fbits (SUC t)).WB.WB_opc = 5w ==>
     (agp32 fext fbits (SUC t)).data_addr = mem_data_addr (FUNPOW Next (THE (I (5,SUC t)) − 1) a)
 Proof
-  rw [] >> Q.ABBREV_TAC `s = agp32 fext fbits t` >>
-  `(agp32 fext fbits (SUC t)).data_addr = (agp32_next_state (fext t) s s).data_addr`
-    by fs [agp32_data_addr_wstrb_wdata_updated_by_agp32_next_state] >>
-  `(fext t).error = 0w` by fs [is_mem_def,mem_no_errors_def] >>
-  `s.MEM.MEM_read_mem` by METIS_TAC [Abbr `s`,agp32_MEM_read_mem_MEM_opc_4w_5w] >>
-  `enable_stg 5 s` by fs [Abbr `s`,enable_stg_def,agp32_MEM_state_flag_eq_WB_state_flag] >>
-  `I' (5,SUC t) = I' (4,t)` by fs [is_sch_def,is_sch_writeback_def] >>
-  `s.state = 0w`
-    by (fs [Abbr `s`,enable_stg_def] >> Cases_on_word_value `(agp32 fext fbits t).state` >>
-        METIS_TAC [agp32_MEM_state_flag_and_state,agp32_state_impossible_values]) >>
-  `(fext t).ready`
-    by (fs [Abbr `s`,enable_stg_def] >> METIS_TAC [agp32_MEM_state_flag_and_fext_ready]) >>
-  fs [agp32_next_state_def] >>
-  `~s.MEM.MEM_isInterrupt` by fs [Abbr `s`,agp32_MEM_read_mem_others_F] >> fs [] >>
-  Cases_on `I' (4,t) = NONE` >-
-   fs [Rel_def,Inv_Rel_def] >>
-  `opc (FUNPOW Next (THE (I' (4,t)) − 1) a) = 5w` by fs [Rel_def,MEM_Rel_def] >>           
-  fs [mem_data_addr_def,Rel_def,MEM_Rel_def]
-QED
-
-
-(** command **)
-Theorem agp32_Rel_ag32_data_addr_correct_MEM_read_mem:
-  !fext fbits a t I.
-    is_mem fext_accessor_circuit (agp32 fext fbits) fext ==>
-    is_sch I (agp32 fext fbits) a ==>
-    Rel I (fext t) (agp32 fext fbits (t-1)) (agp32 fext fbits t) a t ==>
-    (agp32 fext fbits t).MEM.MEM_read_mem ==>
-    enable_stg 4 (agp32 fext fbits t) ==>
-    (agp32 fext fbits (SUC t)).command = 2w
-Proof
-  rw [] >> Q.ABBREV_TAC `s = agp32 fext fbits t` >>
-  `(agp32 fext fbits (SUC t)).command = (agp32_next_state (fext t) s s).command`
-    by fs [agp32_command_state_updated_by_agp32_next_state] >>
-  `(fext t).error = 0w` by fs [is_mem_def,mem_no_errors_def] >>
-  `s.state = 0w`
-    by (fs [Abbr `s`,enable_stg_def] >> Cases_on_word_value `(agp32 fext fbits t).state` >>
-        METIS_TAC [agp32_MEM_state_flag_and_state,agp32_state_impossible_values]) >>
-  `(fext t).ready`
-    by (fs [Abbr `s`,enable_stg_def] >> METIS_TAC [agp32_MEM_state_flag_and_fext_ready]) >>
-  fs [agp32_next_state_def] >>
-  `~s.MEM.MEM_isInterrupt` by fs [Abbr `s`,agp32_MEM_read_mem_others_F] >> fs []
+  rw [] >> Cases_on `enable_stg 5 (agp32 fext fbits t)` >-
+   (Q.ABBREV_TAC `s = agp32 fext fbits t` >>              
+    `(agp32 fext fbits (SUC t)).data_addr = (agp32_next_state (fext t) s s).data_addr`
+      by fs [agp32_data_addr_wstrb_wdata_updated_by_agp32_next_state] >>
+    `(fext t).error = 0w` by fs [is_mem_def,mem_no_errors_def] >>
+    `s.MEM.MEM_opc = 5w` by fs [agp32_WB_opc_MEM_opc_when_WB_enabled,Abbr `s`] >>
+    `s.MEM.MEM_read_mem` by METIS_TAC [Abbr `s`,agp32_MEM_read_mem_MEM_opc_4w_5w] >>
+    `I' (5,SUC t) = I' (4,t)` by fs [is_sch_def,is_sch_writeback_def] >>
+    `s.state = 0w`
+      by (fs [Abbr `s`,enable_stg_def] >> Cases_on_word_value `(agp32 fext fbits t).state` >>
+          METIS_TAC [agp32_WB_state_flag_and_state,agp32_state_impossible_values]) >>
+    `(fext t).ready`
+      by (fs [Abbr `s`,enable_stg_def] >> METIS_TAC [agp32_WB_state_flag_and_fext_ready]) >>
+    fs [agp32_next_state_def] >>
+    `~s.MEM.MEM_isInterrupt` by fs [Abbr `s`,agp32_MEM_read_mem_others_F] >> fs [] >>
+    `opc (FUNPOW Next (THE (I' (4,t)) − 1) a) = 5w` by fs [Rel_def,MEM_Rel_def] >>
+    fs [mem_data_addr_def,Rel_def,MEM_Rel_def]) >>
+  `(agp32 fext fbits (SUC t)).data_addr = (agp32 fext fbits t).data_addr` by cheat >>
+  `I' (5,SUC t) = I' (5,t)` by fs [is_sch_def,is_sch_disable_def] >>
+  `(agp32 fext fbits t).WB.WB_opc = 5w` by fs [agp32_WB_opc_unchanged_when_WB_disabled] >>
+  fs [Rel_def,MEM_req_rel_def]
 QED
     
 
@@ -554,9 +536,10 @@ Theorem agp32_Rel_ag32_MEM_req_rel_correct:
     is_sch I (agp32 fext fbits) a ==>
     Rel I (fext t) (agp32 fext fbits (t-1)) (agp32 fext fbits t) a t ==>
     I (5,SUC t) <> NONE ==>
-    MEM_reg_rel (fext (SUC t)) (agp32 fext fbits t) (agp32 fext fbits (SUC t)) a (THE (I (5,SUC t)))
+    MEM_req_rel (fext (SUC t)) (agp32 fext fbits t) (agp32 fext fbits (SUC t)) a (THE (I (5,SUC t)))
 Proof
   rw [MEM_req_rel_def] >>
+  fs [agp32_Rel_ag32_data_addr_correct_read_mem,agp32_Rel_ag32_data_addr_correct_read_mem_byte] >>
   cheat
 QED
 
